Functional small step cover semantics

Cover.v
@@ -1,5 +1,6 @@
 Require Import PeanoNat.
 Require Import Coq.Arith.Wf_nat.
+Require Import Coq.Relations.Relation_Operators.
 From mathcomp Require Import all_ssreflect.
 Require Import Types.
 
@@ -106,87 +107,498 @@ Arguments Cover [Constructor].
 Arguments ContinueCover [Constructor].
 Hint Constructors Instruction.
 
-
-(*
-
-
-  Definition changedCover
-             (covered: seq (@IT Constructor))
-             (toCover: seq (@IT Constructor)): option (seq (@IT Constructor)) :=
-    let (coveredFresh, uncovered) := paritionCover covered toCover in
-    if coveredFresh is [::] then None else Some uncovered.
-
-Fixpoint cover (splits : seq (MultiArrow * seq (@IT Constructor)))
-           (toCover : seq (@IT Constructor))
-           (currentResult : option MultiArrow)
-           (Delta: seq MultiArrow): seq MultiArrow :=
-    if splits is [:: (srcs, tgt, covered) & splits]
-    then
-      match changedCover covered toCover, currentResult with
-      | Some [::], None =>
-        [:: (srcs, tgt) & cover splits toCover currentResult Delta]
-      | Some [::], Some result =>
-        [:: (mergeMultiArrow result srcs tgt) & cover splits toCover currentResult Delta]
-      | Some remaining, Some (currentSources, currentTarget) =>
-        if all (fun AB => checkSubtypes _ AB.1 AB.2) (zip currentSources srcs)
-        then cover splits remaining (Some (currentSources, tgt \cap currentTarget)) Delta
-        else
-          cover splits remaining
-                       (Some (mergeMultiArrow (currentSources, currentTarget) srcs tgt))
-                       (cover splits toCover currentResult Delta)
-      | Some remaining, None =>
-        cover splits remaining (Some (srcs, tgt))
-              (cover splits toCover currentResult Delta)
-      | None, _ =>
-        cover splits toCover currentResult Delta
-      end
-    else Delta.
-*)
-
+Definition dcap {Constructor: ctor} (A B: @IT Constructor): @IT Constructor :=
+  if checkSubtypes A B
+  then A
+  else if checkSubtypes B A
+       then B
+       else A \cap B.
+Notation "A \dcap B" := (Inter A B) (at level 80, right associativity) : it_scope.
 
 (** A machine a machine covering paths with multi arrows **)
 Section CoverMachine.
   Variable Constructor: ctor.
 
-  Fixpoint paritionCover
+  Fixpoint partitionCover
              (covered: seq (@IT Constructor))
              (toCover: seq (@IT Constructor)): seq (@IT Constructor) * seq (@IT Constructor) :=
     match toCover with
     | [::] => ([::], [::])
     | [:: A & Delta ] =>
-      let (coveredFresh, uncovered) := paritionCover covered Delta in
+      let (coveredFresh, uncovered) := partitionCover covered Delta in
       if A \in covered
       then ([:: A & coveredFresh], uncovered)
       else (coveredFresh, [:: A & uncovered])
-    end.
+    end. 
+
+  Definition mergeMultiArrow
+             (arrow: MultiArrow)
+             (srcs: seq (@IT Constructor))
+             (tgt: @IT Constructor): MultiArrow :=
+    (map (fun src => src.1 \dcap src.2) (zip srcs arrow.1), tgt \cap arrow.2).
 
   (** Small step semantics of the cover machine **)
-  Inductive StepSemantics :
-    @State Constructor * seq (@Instruction Constructor) -> (@State Constructor) * seq (@Instruction Constructor) -> Prop :=
+  Inductive StepSemantics:
+    @State Constructor * seq (@Instruction Constructor) ->
+    @State Constructor * seq (@Instruction Constructor) -> Prop :=
   | step__done: forall s toCover p,
       (s, [:: Cover [::] toCover & p]) ~~> (s, p)
   | step__doneContinue: forall s toCover currentResult p,
       (s, [:: ContinueCover [::] toCover currentResult & p]) ~~> (s, p)
-  | step__skip: forall s src tgt covered splits toCover p,
-      ((paritionCover covered toCover).1 == [::]) ->
-      (s, [:: Cover [:: (src, tgt, covered) & splits] toCover & p]) ~~> (s, [:: Cover splits toCover & p])
-  | step__skipContinue: forall s src tgt covered splits toCover currentResult p,
-      ((paritionCover covered toCover).1 == [::]) ->
-      (s, [:: ContinueCover [:: (src, tgt, covered) & splits] toCover currentResult & p])
+  | step__skip: forall s srcs tgt covered splits toCover p,
+      ((partitionCover covered toCover).1 == [::]) ->
+      (s, [:: Cover [:: (srcs, tgt, covered) & splits] toCover & p])
+        ~~> (s, [:: Cover splits toCover & p])
+  | step__skipContinue: forall s srcs tgt covered splits toCover currentResult p,
+      ((partitionCover covered toCover).1 == [::]) ->
+      (s, [:: ContinueCover [:: (srcs, tgt, covered) & splits] toCover currentResult & p])
         ~~> (s, [:: ContinueCover splits toCover currentResult & p])
+  | step__addDone: forall s srcs tgt covered splits toCover p,
+      ((partitionCover covered toCover).1 != [::]) ->
+      ((partitionCover covered toCover).2 == [::]) ->
+      (s, [:: Cover [:: (srcs, tgt, covered) & splits] toCover & p])
+        ~~> ([:: (srcs, tgt) & s], [:: Cover splits toCover & p])
+  | step__mergeDone:
+      forall s srcs tgt covered splits toCover currentResult p,
+      ((partitionCover covered toCover).1 != [::]) ->
+      ((partitionCover covered toCover).2 == [::]) ->
+      (s, [:: ContinueCover [:: (srcs, tgt, covered) & splits] toCover currentResult & p])
+        ~~> ( [:: mergeMultiArrow currentResult srcs tgt & s]
+            , [:: ContinueCover splits toCover currentResult & p])
+  | step__continue:
+      forall s srcs tgt covered splits toCover p,
+        ((partitionCover covered toCover).1 != [::]) ->
+        ((partitionCover covered toCover).2 != [::]) ->
+        (s, [:: Cover [:: (srcs, tgt, covered) & splits] toCover & p])
+          ~~> ( s
+              , [:: ContinueCover splits (partitionCover covered toCover).2 (srcs, tgt)
+                 , Cover splits toCover 
+                   & p])
+  | step__continueMergeAlways:
+      forall s srcs tgt covered splits toCover currentResult p,
+        ((partitionCover covered toCover).1 != [::]) ->
+        ((partitionCover covered toCover).2 != [::]) ->
+        ((mergeMultiArrow currentResult srcs tgt).1 == currentResult.1) ->
+        (s, [:: ContinueCover [:: (srcs, tgt, covered) & splits] toCover currentResult & p])
+          ~~> (s
+             , [:: ContinueCover
+                   splits (partitionCover covered toCover).2
+                   (mergeMultiArrow currentResult srcs tgt)
+                & p])
+  | step__continueMergeOptions:
+      forall s srcs tgt covered splits toCover currentResult p,
+        ((partitionCover covered toCover).1 != [::]) ->
+        ((partitionCover covered toCover).2 != [::]) ->
+        ((mergeMultiArrow currentResult srcs tgt).1 != currentResult.1) ->
+        (s, [:: ContinueCover [:: (srcs, tgt, covered) & splits] toCover currentResult & p])
+          ~~> (s
+             , [:: ContinueCover
+                   splits (partitionCover covered toCover).2
+                   (mergeMultiArrow currentResult srcs tgt)
+                , ContinueCover splits toCover currentResult
+                & p])
   where "p1 ~~> p2" := (StepSemantics p1 p2).
+
+  Definition Semantics := clos_trans_1n _ StepSemantics.
 End CoverMachine.
+
+
+Arguments partitionCover [Constructor].
+Arguments mergeMultiArrow [Constructor].
 
 Arguments StepSemantics [Constructor].
 Arguments step__done [Constructor s toCover p].
 Arguments step__doneContinue [Constructor s toCover currentResult p].
-Arguments step__Arr [Constructor A B1 B2 Delta r].
-Arguments step__chooseTgt [Constructor B A Delta Delta' r].
-Arguments step__doneTgt [Constructor B].
-Arguments step__Prod [Constructor A B1 B2 r1 r2].
-Arguments step__Inter [Constructor A B1 B2 r1 r2].
-Hint Constructors Semantics.
-Notation "p1 ~~> p2" := (Semantics p1 p2).
+Arguments step__skip [Constructor s srcs tgt covered splits toCover p].
+Arguments step__skipContinue [Constructor s srcs tgt covered splits toCover currentResult p].
+Arguments step__addDone [Constructor s srcs tgt covered splits toCover p].
+Arguments step__mergeDone [Constructor s srcs tgt covered splits toCover currentResult p].
+Arguments step__continue [Constructor s srcs tgt covered splits toCover p].
+Arguments step__continueMergeAlways [Constructor s srcs tgt covered splits toCover currentResult p].
+Arguments step__continueMergeOptions [Constructor s srcs tgt covered splits toCover currentResult p].
+Hint Constructors StepSemantics.
 
-Arguments slow_cast [Constructor].
-Arguments cast [Constructor].
+Arguments Semantics [Constructor].
+
+Notation "p1 ~~> p2" := (StepSemantics p1 p2).
+Notation "p1 '~~>[+]' p2" := (Semantics p1 p2) (at level 70, no associativity) : it_scope.
+
+(** Small step inversion for the cover machine **)
+Section CoverMachineInversion.
+  Variable Constructor: ctor.
+
+  Definition CoverMachine_inv
+             {sp1 sp2: @State Constructor * seq (@Instruction Constructor)}
+             (prf: sp1 ~~> sp2)
+             (X: @State Constructor * seq (@Instruction Constructor) ->
+                 @State Constructor * seq (@Instruction Constructor) -> Prop) :=
+    let diag (x y: @State Constructor *  seq (@Instruction Constructor)): Prop :=
+        let (s1, p1) := x in
+        let (s2, p2) := y in
+        match p1 return Prop with
+        |  [:: Cover [::] toCover & p1] =>
+           (X (s1, [:: Cover [::] toCover & p1]) (s1, p1) ->
+            X (s1, [:: Cover [::] toCover & p1]) (s2, p2))%type
+        | [:: ContinueCover [::] toCover currentResult & p1] =>
+          (X (s1, [:: ContinueCover [::] toCover currentResult & p1]) (s1, p1) ->
+           X (s1, [:: ContinueCover [::] toCover currentResult & p1]) (s2, p2))%type
+        | [:: Cover [:: (srcs, tgt, covered) & splits] toCover & p1] =>
+          ((((partitionCover covered toCover).1 == [::]) ->
+            X (s1, [:: Cover [:: (srcs, tgt, covered) & splits] toCover & p1])
+              (s1, [:: Cover splits toCover & p1])) ->
+           (((partitionCover covered toCover).1 != [::]) ->
+            ((partitionCover covered toCover).2 == [::]) ->
+            X (s1, [:: Cover [:: (srcs, tgt, covered) & splits] toCover & p1])
+              ([:: (srcs, tgt) & s1], [:: Cover splits toCover & p1])) ->
+           (((partitionCover covered toCover).1 != [::]) ->
+            ((partitionCover covered toCover).2 != [::]) ->
+            X (s1, [:: Cover [:: (srcs, tgt, covered) & splits] toCover & p1])
+              (s1, [:: ContinueCover splits (partitionCover covered toCover).2 (srcs, tgt)
+                    , Cover splits toCover 
+                      & p1])) ->
+           X (s1, [:: Cover [:: (srcs, tgt, covered) & splits] toCover & p1]) (s2, p2))%type
+        | [:: ContinueCover [:: (srcs, tgt, covered) & splits] toCover currentResult & p1] =>
+          ((((partitionCover covered toCover).1 == [::]) ->
+            X (s1, [:: ContinueCover [:: (srcs, tgt, covered) & splits] toCover currentResult & p1])
+              (s1, [:: ContinueCover splits toCover currentResult & p1])) ->
+           (((partitionCover covered toCover).1 != [::]) ->
+            ((partitionCover covered toCover).2 == [::]) ->
+            X (s1, [:: ContinueCover [:: (srcs, tgt, covered) & splits] toCover currentResult & p1])
+              ([:: mergeMultiArrow currentResult srcs tgt & s1]
+               , [:: ContinueCover splits toCover currentResult & p1])) ->
+           (((partitionCover covered toCover).1 != [::]) ->
+            ((partitionCover covered toCover).2 != [::]) ->
+            ((mergeMultiArrow currentResult srcs tgt).1 == currentResult.1) ->
+            X (s1, [:: ContinueCover [:: (srcs, tgt, covered) & splits] toCover currentResult & p1])
+              (s1
+               , [:: ContinueCover
+                     splits (partitionCover covered toCover).2
+                     (mergeMultiArrow currentResult srcs tgt)
+                  & p1])) ->
+           (((partitionCover covered toCover).1 != [::]) ->
+            ((partitionCover covered toCover).2 != [::]) ->
+            ((mergeMultiArrow currentResult srcs tgt).1 != currentResult.1) ->
+            X (s1, [:: ContinueCover [:: (srcs, tgt, covered) & splits] toCover currentResult & p1])
+              (s1
+               , [:: ContinueCover
+                     splits (partitionCover covered toCover).2
+                     (mergeMultiArrow currentResult srcs tgt)
+                  , ContinueCover splits toCover currentResult
+                    & p1])) ->
+           X (s1, [:: ContinueCover [:: (srcs, tgt, covered) & splits] toCover currentResult & p1]) (s2, p2))%type
+        | _ => False
+        end in
+    match prf in x ~~> y return diag x y with
+    | step__done s toCover p =>
+      fun k => k
+    | step__doneContinue s toCover currentResult p =>
+      fun k => k
+    | step__skip s srcs tgt covered splits toCover p noFresh =>
+      fun k _ _ => k noFresh
+    | step__skipContinue s srcs tgt covered splits toCover currentResult p noFresh =>
+      fun k _ _ _ => k noFresh
+    | step__addDone s srcs tgt covered splits toCover p fresh noLeft =>
+      fun _ k _ => k fresh noLeft
+    | step__mergeDone s srcs tgt covered splits toCover currentResult p fresh noLeft =>
+      fun _ k _ _ => k fresh noLeft
+    | step__continue s srcs tgt covered splits toCover p fresh someLeft =>
+      fun _ _ k => k fresh someLeft
+    | step__continueMergeAlways s srcs tgt covered splits toCover currentResult p fresh someLeft redundant =>
+      fun _ _ k _ => k fresh someLeft redundant
+    | step__continueMergeOptions s srcs tgt covered splits toCover currentResult p fresh someLeft notRedundant =>
+      fun _ _ _ k => k fresh someLeft notRedundant
+    end.
+
+End CoverMachineInversion.
+
+Arguments CoverMachine_inv [Constructor] [sp1 sp2].
+
+Section CoverMachineProperties.
+  Variable Constructor: ctor.
+  Implicit Type p: seq (@Instruction Constructor).
+  Implicit Type s: @State Constructor.
+  Implicit Type sp: @State Constructor * seq (@Instruction Constructor).
+
+  Lemma coverMachineFunctional_step:
+    forall sp sp1 sp2, sp ~~> sp1 -> sp ~~> sp2 -> sp1 = sp2.
+  Proof.
+    move => [] s p [] s1 p1 [] s2 p2 prf1.
+    move: (CoverMachine_inv prf1 (fun x y => (x ~~> (s2, p2) -> y = (s2, p2))%type)).
+    move: prf1 => _.
+    case: p => //=.
+    case => //=.
+    case => //=.
+    - move => toCover p res.
+      apply: res.
+      move => /CoverMachine_inv res'.
+        by apply: (res' (fun x y => (s, p) = y)%type).
+    - move => [] [] srcs tgt covered splits toCover p res.
+      apply: res.
+      + move => noFresh.
+        move => /CoverMachine_inv res'.
+        apply: (res' (fun x y => _ = y)%type) => //;
+          by rewrite noFresh.
+      + move => fresh noLeft.
+        move => /CoverMachine_inv res'.
+        apply: (res' (fun x y => _ = y)%type) => //.
+        * move => noFresh.
+          move: fresh.
+            by rewrite noFresh.
+        * by rewrite noLeft.
+      + move => fresh someLeft.
+        move => /CoverMachine_inv res'.
+        apply: (res' (fun x y => _ = y)%type) => //.
+        * move => noFresh.
+          move: fresh.
+            by rewrite noFresh.
+        * move => _ noLeft.
+          move: someLeft.
+            by rewrite noLeft.
+    - case.
+      + move => toCover currentResult p res.
+        apply: res.
+        move => /CoverMachine_inv res'.
+          by apply: (res' (fun x y => (s, p) = y)%type).
+      + move => [] [] srcs tgt covered splits toCover currentResult p res.
+        apply: res.
+        * move => noFresh.
+          move => /CoverMachine_inv res'.
+          apply: (res' (fun x y => _ = y)%type) => //;
+            by rewrite noFresh.
+        * move => fresh noLeft.
+          move => /CoverMachine_inv res'.
+          apply: (res' (fun x y => _ = y)%type) => //; try by rewrite noLeft.
+          move => noFresh.
+          move: fresh.
+            by rewrite noFresh.
+        * move => fresh someLeft redundant.
+          move => /CoverMachine_inv res'.
+          apply: (res' (fun x y => _ = y)%type) => //.
+          ** move => noFresh.
+             move: fresh.
+               by rewrite noFresh.
+          ** move => _ noLeft.
+             move: someLeft.
+               by rewrite noLeft.
+          ** by rewrite redundant.
+        * move => fresh someLeft notRedundant.
+          move => /CoverMachine_inv res'.
+          apply: (res' (fun x y => _ = y)%type) => //.
+          ** move => noFresh.
+             move: fresh.
+               by rewrite noFresh.
+          ** move => _ noLeft.
+             move: someLeft.
+               by rewrite noLeft.
+          ** move => _ _ redundant.
+             move: notRedundant.
+               by rewrite redundant.
+  Qed.
+
+  Reserved Notation "p1 '~~>[' n ']' p2" (at level 70, no associativity).
+  Inductive nStepSemantics:
+    nat -> 
+    @State Constructor * seq (@Instruction Constructor) ->
+    @State Constructor * seq (@Instruction Constructor) -> Prop :=
+  | LastStep: forall sp1 sp2,
+      sp1 ~~> sp2 ->
+      sp1 ~~>[1] sp2
+  | MoreSteps: forall n sp1 sp2 sp3,
+      sp1 ~~> sp2 ->
+      sp2 ~~>[n.+1] sp3 ->
+      sp1 ~~>[n.+2] sp3
+  where "sp1 '~~>[' n ']' sp2" := (nStepSemantics n sp1 sp2).
+  Hint Constructors nStepSemantics.
+
+  Lemma nStepSemantics_sound: forall n s1 p1 s2 p2,
+      (s1, p1) ~~>[n] (s2, p2) ->
+      (s1, p1) ~~>[+] (s2, p2).
+  Proof.
+    move => n s1 p1 s2 p2.
+    elim.
+    - move => *.
+        by apply: t1n_step.
+    - move => ? ? ? ? prf *.
+        by apply: t1n_trans; first by exact prf.
+  Qed.
+
+  Lemma nStepSemantics_complete:
+    forall sp1 sp2,
+      sp1 ~~>[+] sp2 ->
+      exists n, sp1 ~~>[n] sp2.
+  Proof.
+    move => sp1 sp2 prf.
+    elim: sp1 sp2 / prf.
+    - move => sp1 sp2 prf.
+      exists 1.
+        by apply LastStep.
+    - move => sp1 sp2 sp3 prf _ [] n prfs.
+      exists (n.+1).
+      move: prf.
+      case: n sp2 sp3 / prfs.
+      + move => ? ? ? prf.
+        apply: MoreSteps; first by exact prf.
+          by apply: LastStep.
+      + move => ? ? ? ? prf1 ? prf2.
+        apply: MoreSteps; first by exact prf2.
+          by apply: MoreSteps; first by exact prf1.
+  Qed.
+
+  Definition nStepSemantics_inv n sp1 sp2 (prf: sp1 ~~>[n] sp2)
+             (X: nat ->
+                 @State Constructor * seq (@Instruction Constructor) ->
+                 @State Constructor * seq (@Instruction Constructor) -> Prop) :=
+    let diag n sp1 sp2 :=
+        match n return Prop with
+        | 0 => False
+        | 1 =>
+          ((sp1 ~~> sp2 -> X 1 sp1 sp2) -> X 1 sp1 sp2)%type
+        | n.+2 =>
+          (((forall sp3, sp1 ~~> sp3 -> sp3 ~~>[n.+1] sp2 -> X (n.+2) sp1 sp2)%type) ->
+           X (n.+2) sp1 sp2)%type
+        end in
+    match prf in sp1 ~~>[n] sp2 return diag n sp1 sp2 with
+    | LastStep _ _ prf => fun k => k prf
+    | MoreSteps _ _ _ _ prf1 prf2 =>
+      fun k => k _ prf1 prf2
+    end.
+  
+  Lemma coverMachineFunctional:
+    forall n sp sp1 sp2, sp ~~>[n] sp1 -> sp ~~>[n] sp2 -> sp1 = sp2.
+  Proof.
+    move => n sp sp1 sp2 prf1.
+    move: sp2.
+    elim: n sp sp1 / prf1.
+    - move => sp1 sp2 prf1 sp3 /nStepSemantics_inv res.
+      apply: (res (fun _ _ sp3 => sp2 = sp3)) => prf2.
+        by apply: coverMachineFunctional_step; first by exact prf1.
+    - move => n sp1 sp2 sp3 prf prfs IH sp4 /nStepSemantics_inv res.
+      apply: (res (fun _ _ sp4 => sp3 = sp4)).
+        by move => sp2' /(coverMachineFunctional_step _ _ _ prf) <- /IH.
+  Qed.
+
+  (** The set of instructions from the domain of the cover machine relation,
+       i.e. { (s, p) | exists s', (s, p) ~~>[+] (s', [::]) } **)
+  Inductive Domain: @State Constructor * seq (@Instruction Constructor) -> Prop :=
+  | dom__doneEmpty: forall s toCover,
+      Domain (s, [:: Cover [::] toCover])
+  | dom__done: forall s toCover p,
+      Domain (s, p) ->
+      Domain (s, [:: Cover [::] toCover & p])
+  | dom__doneContinueEmpty: forall s toCover currentResult,
+      Domain (s, [:: ContinueCover [::] toCover currentResult ])
+  | dom__doneContinue: forall s toCover currentResult p,
+      Domain (s, p) ->
+      Domain (s, [:: ContinueCover [::] toCover currentResult & p])
+  | dom__skip: forall s srcs tgt covered splits toCover p,
+      ((partitionCover covered toCover).1 == [::]) ->
+      Domain (s, [:: Cover splits toCover & p]) ->
+      Domain (s, [:: Cover [:: (srcs, tgt, covered) & splits] toCover & p])
+  | dom__skipContinue: forall s srcs tgt covered splits toCover currentResult p,
+      ((partitionCover covered toCover).1 == [::]) ->
+      Domain (s, [:: ContinueCover splits toCover currentResult & p]) ->
+      Domain (s, [:: ContinueCover [:: (srcs, tgt, covered) & splits] toCover currentResult & p])
+  | dom__addDone: forall s srcs tgt covered splits toCover p,
+      ((partitionCover covered toCover).1 != [::]) ->
+      ((partitionCover covered toCover).2 == [::]) ->
+      Domain ([:: (srcs, tgt) & s], [:: Cover splits toCover & p]) ->
+      Domain (s, [:: Cover [:: (srcs, tgt, covered) & splits] toCover & p])
+  | dom__mergeDone:
+      forall s srcs tgt covered splits toCover currentResult p,
+      ((partitionCover covered toCover).1 != [::]) ->
+      ((partitionCover covered toCover).2 == [::]) ->
+      Domain ([:: mergeMultiArrow currentResult srcs tgt & s]
+              , [:: ContinueCover splits toCover currentResult & p]) ->
+      Domain (s, [:: ContinueCover [:: (srcs, tgt, covered) & splits] toCover currentResult & p])
+  | dom__continue:
+      forall s srcs tgt covered splits toCover p,
+        ((partitionCover covered toCover).1 != [::]) ->
+        ((partitionCover covered toCover).2 != [::]) ->
+        Domain ( s
+                 , [:: ContinueCover splits (partitionCover covered toCover).2 (srcs, tgt)
+                    , Cover splits toCover 
+                      & p]) ->
+        Domain (s, [:: Cover [:: (srcs, tgt, covered) & splits] toCover & p])
+  | dom__continueMergeAlways:
+      forall s srcs tgt covered splits toCover currentResult p,
+        ((partitionCover covered toCover).1 != [::]) ->
+        ((partitionCover covered toCover).2 != [::]) ->
+        ((mergeMultiArrow currentResult srcs tgt).1 == currentResult.1) ->
+        Domain (s
+                , [:: ContinueCover
+                      splits (partitionCover covered toCover).2
+                      (mergeMultiArrow currentResult srcs tgt)
+                   & p]) ->
+        Domain (s, [:: ContinueCover [:: (srcs, tgt, covered) & splits] toCover currentResult & p])
+  | dom__continueMergeOptions:
+      forall s srcs tgt covered splits toCover currentResult p,
+        ((partitionCover covered toCover).1 != [::]) ->
+        ((partitionCover covered toCover).2 != [::]) ->
+        ((mergeMultiArrow currentResult srcs tgt).1 != currentResult.1) ->
+        Domain (s
+                , [:: ContinueCover
+                      splits (partitionCover covered toCover).2
+                      (mergeMultiArrow currentResult srcs tgt)
+                   , ContinueCover splits toCover currentResult
+                     & p]) ->
+        Domain (s, [:: ContinueCover [:: (srcs, tgt, covered) & splits] toCover currentResult & p]).
+
+  Arguments dom__doneEmpty [s toCover].
+  Arguments dom__done [s toCover p].
+  Arguments dom__doneContinueEmpty [s toCover currentResult].
+  Arguments dom__doneContinue [s toCover currentResult p].
+  Arguments dom__skip [s srcs tgt covered splits toCover p].
+  Arguments dom__skipContinue [s srcs tgt covered splits toCover currentResult p].
+  Arguments dom__addDone [s srcs tgt covered splits toCover p].
+  Arguments dom__mergeDone [s srcs tgt covered splits toCover currentResult p].
+  Arguments dom__continue [s srcs tgt covered splits toCover p].
+  Arguments dom__continueMergeAlways [s srcs tgt covered splits toCover currentResult p].
+  Arguments dom__continueMergeOptions [s srcs tgt covered splits toCover currentResult p].
+  Hint Constructors Domain.
+
+  Definition splitsOf (i: @Instruction Constructor) :=
+    match i with
+    | Cover splits _ => splits
+    | ContinueCover splits _ _ => splits
+    end.
+
+  Definition sumOfSplits p : nat :=
+    \sum_(i <- p) ((seq.size (splitsOf i)).+1).
+
+  Lemma coverMachine_total: forall s i p, Domain (s, [:: i & p]).
+  Proof.
+    move => s i p.
+    move: s.
+    apply: (fun res => induction_ltof1 _
+                                    (fun ip => sumOfSplits [:: ip.1 & ip.2])
+                                    (fun ip => forall s, Domain (s, [:: ip.1 & ip.2]))
+                                    res (i, p)).
+    move: i p => _ _ [] [] [].
+    - move => toCover [] //= i p IH s.
+      apply: dom__done.
+      apply: (IH (i, p)).
+        by rewrite /ltof /sumOfSplits unlock //=.
+    - move => [] [] srcs tgt covered splits toCover p IH s.
+      case fresh: (partitionCover covered toCover).1.
+      + apply: dom__skip; first by rewrite fresh.
+        apply: (IH (_, p)).
+          by rewrite /ltof /sumOfSplits unlock //=.
+      + case left: (partitionCover covered toCover).2.
+        * apply: dom__addDone.
+          ** by rewrite fresh.
+          ** by rewrite left.
+          ** apply: (IH (_, p)).
+               by rewrite /ltof /sumOfSplits unlock //=.
+        * apply: dom__continue.
+          ** by rewrite fresh.
+          ** by rewrite left.
+          ** rewrite /=.
+             apply: (IH (_, p)).
+               by rewrite /ltof /sumOfSplits unlock //=.
+
+
+
+  
+    
+
+
